Weidenbach_Book/Watched_Literals_Watch_List_Restart.thy
@@ -1548,6 +1548,7 @@ definition cdcl_twl_full_restart_wl_GC_prog_post :: \<open>'v twl_st_wl \<Righta
 
 definition cdcl_twl_full_restart_wl_GC_prog where
 \<open>cdcl_twl_full_restart_wl_GC_prog S = do {
+    S \<leftarrow> cdcl_twl_local_restart_wl_spec S;
     T \<leftarrow> remove_one_annot_true_clause_imp_wl S;
     ASSERT(mark_to_delete_clauses_wl_pre T);
     U \<leftarrow> mark_to_delete_clauses_wl T;
